qed auditor checkUpd

src/program_proof/pav/auditor.v
@@ -2,6 +2,7 @@ From Perennial.program_proof Require Import grove_prelude.
 From Goose.github_com.mit_pdos.pav Require Import kt.
 
 From Perennial.program_proof.pav Require Import core cryptoffi merkle serde.
+From Perennial.Helpers Require Import Map.
 
 Section gs.
 Context `{!heapGS Σ, !pavG Σ}.
@@ -73,7 +74,7 @@ Context `{!heapGS Σ, !pavG Σ}.
 
 Lemma wp_NewAuditor :
   {{{
-        True
+    True
   }}}
   NewAuditor #()
   {{{
@@ -108,71 +109,13 @@ Proof.
   by iApply own_slice_small_nil.
 Qed.
 
-Lemma wp_Auditor__Update a ptr_upd upd :
-  {{{
-        "#Hvalid" ∷ Auditor.valid a ∗
-        "Hupdate" ∷ UpdateProof.own ptr_upd upd
-  }}}
-  Auditor__Update #a #ptr_upd
-  {{{
-        (e : bool), RET #e; True
-  }}}.
-Proof.
-  iIntros (?) "H HΦ". iNamed "H".
-  iNamed "Hvalid".
-  wp_rec. wp_pures.
-  wp_loadField.
-  wp_apply (wp_Mutex__Lock with "[$]").
-  iIntros "[Hlock Hown]".
-  iNamed "Hown".
-  wp_pures.
-  wp_loadField.
-  wp_apply wp_slice_len.
-  wp_pures.
-  iNamed "Hupdate".
-  wp_loadField.
-
-  (* XXX: checkUpd only gets called here. Inlining its proof. *)
-  wp_rec.
-  wp_pures.
-  wp_loadField.
-  wp_apply wp_slice_len.
-  wp_pures.
-  wp_apply wp_ref_of_zero.
-  { done. }
-  iIntros (?) "Hl".
-  wp_pures.
-  wp_apply (wp_MapIter_fold _ _ _ (λ _,
-                                     _
-              )%I with "[$] [-HΦ]").
-  { iNamedAccu. }
-  {
-    iIntros "* !# * [Hpre %Hlookup] HΦ".
-    iNamed "Hpre".
-    wp_pures.
-    wp_apply wp_StringToBytes.
-    iIntros "* ?".
-    iDestruct (own_slice_to_small with "[$]") as "?".
-    (* XXX: checkOneUpd only called here so inlining a proof. *)
-    wp_rec.
-    wp_pures.
-    wp_loadField.
-    wp_apply (wp_Tree_Get with "[$]").
-    iIntros "* HGetPost".
-    iNamed "HGetPost".
-    (* iNamed "Hreply". *)
-    wp_pures.
-    admit.
-  }
-Admitted.
-
 Lemma wp_Auditor__Get a (epoch : u64) :
   {{{
-        "#Hvalid" ∷ Auditor.valid a
+    "#Hvalid" ∷ Auditor.valid a
   }}}
   Auditor__Get #a #epoch
   {{{
-        (b : bool) (p : loc) o, RET (#p, #b); AdtrEpochInfo.own p o
+    (b : bool) (p : loc) o, RET (#p, #b); AdtrEpochInfo.own p o
   }}}.
 Proof.
   iIntros (?) "H HΦ". iNamed "H".
@@ -182,10 +125,8 @@ Proof.
   wp_apply (wp_Mutex__Lock with "[$]").
   iIntros "[Hlock Hown]".
   iNamed "Hown".
-  wp_pures.
   wp_loadField.
   wp_apply wp_slice_len.
-  wp_pures.
   wp_if_destruct.
   - wp_loadField.
     wp_apply (wp_Mutex__Unlock with "[-HΦ]").
@@ -220,5 +161,156 @@ Proof.
     iApply "HΦ".
     by iFrame "#".
 Qed.
+
+Definition upd_checks (keys : adtr_map_ty) (nextEp : w64) (label val : list w8) :=
+  ∃ comm,
+  length label = 32%nat ∧
+  keys !! label = None ∧
+  val = MapValPre.encodesF (MapValPre.mk nextEp comm).
+
+Lemma wp_checkOneUpd ptr_keys keys nextEp sl_label dq label sl_val val :
+  {{{
+    "Hown_keys" ∷ own_merkle ptr_keys (lower_map keys) ∗
+    "Hsl_label" ∷ own_slice_small sl_label byteT dq label ∗
+    "#Hsl_val" ∷ own_slice_small sl_val byteT DfracDiscarded val
+  }}}
+  checkOneUpd #ptr_keys #nextEp (slice_val sl_label) (slice_val sl_val)
+  {{{
+    (err : bool), RET #err;
+    "Hown_keys" ∷ own_merkle ptr_keys (lower_map keys) ∗
+    "Hsl_label" ∷ own_slice_small sl_label byteT dq label ∗
+    "Herr" ∷ (if err then True else ⌜ upd_checks keys nextEp label val ⌝)
+  }}}.
+Proof.
+  iIntros (Φ) "H HΦ". iNamed "H". wp_rec.
+  wp_apply (wp_Tree__Get with "[$Hown_keys $Hsl_label]").
+  iIntros "*". iNamedSuffix 1 "_map".
+  wp_if_destruct. { iApply "HΦ". by iFrame. }
+  wp_if_destruct. { iApply "HΦ". by iFrame. }
+  wp_apply (MapValPre.wp_dec with "[$Hsl_val]").
+  iIntros "*". iNamedSuffix 1 "_val".
+  wp_if_destruct. { iApply "HΦ". by iFrame. }
+  wp_apply wp_slice_len.
+  wp_if_destruct. { iApply "HΦ". by iFrame. }
+  iDestruct ("Herr_val" with "[//]") as "H".
+  iNamedSuffix "H" "_dec". iNamed "Hown_obj_dec".
+  wp_loadField.
+  (* TODO: seal up own_merkle so it doesn't get unfolded by iFrame. *)
+  wp_if_destruct. { iApply "HΦ". by iFrame "Htree_map ∗". }
+  iApply "HΦ". iFrame "Htree_map ∗".
+  iNamedSuffix "Herr_map" "_map".
+  iDestruct (is_merkle_proof_to_entry with "His_proof_map") as "#His_entry".
+  iDestruct (is_merkle_entry_with_map with "His_entry His_dig_map") as %Hlook_keys.
+  iDestruct (own_slice_small_sz with "Hsl_tail_dec") as %Hlen_tail.
+  opose proof (nil_length_inv tail _) as ->; [word|].
+  (* TODO: somehow u64_le now gets unfolded by simpl. *)
+  iPureIntro. eexists. repeat try split; [naive_solver|..].
+  { rewrite lookup_fmap in Hlook_keys. by apply fmap_None in Hlook_keys. }
+  by list_simplifier.
+Qed.
+
+Lemma wp_checkUpd ptr_keys keys ptr_upd upd_refs upd nextEp :
+  {{{
+    "Hown_keys" ∷ own_merkle ptr_keys (lower_map keys) ∗
+    "#Hown_upd_refs" ∷ own_map ptr_upd DfracDiscarded upd_refs ∗
+    "#Hown_upd" ∷ ([∗ map] sl;v ∈ upd_refs;upd,
+      own_slice_small sl byteT DfracDiscarded v)
+  }}}
+  checkUpd #ptr_keys #nextEp #ptr_upd
+  {{{
+    (err : bool), RET #err;
+    "Hown_keys" ∷ own_merkle ptr_keys (lower_map keys) ∗
+    "Herr" ∷ (if err then True else
+      ([∗ map] label ↦ val ∈ upd, ⌜ upd_checks keys nextEp label val ⌝))
+  }}}.
+Proof.
+  iIntros (Φ) "H HΦ". iNamed "H". wp_rec.
+  wp_apply wp_ref_of_zero; [done|]. iIntros (ptr_loopErr) "Hptr_loopErr".
+  wp_apply (wp_MapIter_fold _ _ _
+    (λ upd_refs',
+    ∃ (loopErr : bool),
+    "Hown_keys" ∷ own_merkle ptr_keys (lower_map keys) ∗
+    "Hptr_loopErr" ∷ ptr_loopErr ↦[boolT] #loopErr ∗
+    "HloopErr" ∷ (if loopErr then True else
+      ∃ upd',
+      "%Hdom" ∷ ⌜ dom upd_refs' = dom upd' ⌝ ∗
+      "%Hsub" ∷ ⌜ upd' ⊆ upd ⌝ ∗
+      "%Hchecks" ∷ ([∗ map] label ↦ val ∈ upd', ⌜ upd_checks keys nextEp label val ⌝))
+    )%I with "Hown_upd_refs [$Hown_keys $Hptr_loopErr]").
+  { iExists ∅. repeat try iSplit; try naive_solver.
+    iPureIntro. eapply map_empty_subseteq. }
+  { clear. iIntros (? k sl_v Φ) "!> (H&_&%Hlook_ptr) HΦ". iNamed "H".
+    wp_apply wp_StringToBytes. iIntros (?) "Hsl_label".
+    iDestruct (own_slice_to_small with "Hsl_label") as "Hsl_label".
+    iDestruct (big_sepM2_lookup_l_some with "Hown_upd") as %[v Hlook_val];
+      [exact Hlook_ptr|].
+    iDestruct (big_sepM2_lookup with "Hown_upd") as "#Hsl_val";
+      [exact Hlook_ptr|exact Hlook_val|].
+    wp_apply (wp_checkOneUpd with "[$Hown_keys $Hsl_label $Hsl_val]").
+    iIntros "*". iNamed 1. wp_if_destruct.
+    { wp_store. iApply "HΦ". by iFrame. }
+    iDestruct "Herr" as "%Herr". iApply "HΦ". iFrame.
+    destruct loopErr; [done|]. iNamed "HloopErr".
+    iExists (<[k:=v]> upd'). iPureIntro. repeat try split.
+    - set_solver.
+    - by apply insert_subseteq_l.
+    - by apply map_Forall_insert_2. }
+  iIntros "[_ H]". iNamed "H".
+  wp_load. iApply "HΦ". iFrame. destruct loopErr; [done|]. iNamed "HloopErr".
+  iDestruct (big_sepM2_dom with "Hown_upd") as %Hdom1.
+  opose proof (map_subset_dom_eq _ _ _ _ _ Hsub) as ->; [|done].
+  by rewrite -Hdom -Hdom1.
+Qed.
+
+Lemma wp_Auditor__Update a ptr_upd upd :
+  {{{
+    "#Hvalid" ∷ Auditor.valid a ∗
+    "Hupdate" ∷ UpdateProof.own ptr_upd upd
+  }}}
+  Auditor__Update #a #ptr_upd
+  {{{
+    (e : bool), RET #e; True
+  }}}.
+Proof.
+  iIntros (?) "H HΦ". iNamed "H". iNamed "Hvalid". wp_rec.
+  wp_loadField.
+  wp_apply (wp_Mutex__Lock with "[$]").
+  iIntros "[Hlock H]". iNamed "H".
+  wp_loadField. wp_apply wp_slice_len.
+  iNamed "Hupdate". do 2 wp_loadField.
+
+  (* XXX: checkUpd only gets called here. Inlining its proof. *)
+  wp_rec.
+  wp_pures.
+  wp_loadField.
+  wp_apply wp_slice_len.
+  wp_pures.
+  wp_apply wp_ref_of_zero.
+  { done. }
+  iIntros (?) "Hl".
+  wp_pures.
+  wp_apply (wp_MapIter_fold _ _ _ (λ _,
+                                     _
+              )%I with "[$] [-HΦ]").
+  { iNamedAccu. }
+  {
+    iIntros "* !# * [Hpre %Hlookup] HΦ".
+    iNamed "Hpre".
+    wp_pures.
+    wp_apply wp_StringToBytes.
+    iIntros "* ?".
+    iDestruct (own_slice_to_small with "[$]") as "?".
+    (* XXX: checkOneUpd only called here so inlining a proof. *)
+    wp_rec.
+    wp_pures.
+    wp_loadField.
+    wp_apply (wp_Tree_Get with "[$]").
+    iIntros "* HGetPost".
+    iNamed "HGetPost".
+    (* iNamed "Hreply". *)
+    wp_pures.
+    admit.
+  }
+Admitted.
 
 End specs.
